src/ReactorModel/Execution/Theorems/StateOver.lean
@@ -1,0 +1,61 @@
+import ReactorModel.Execution.Theorems.State
+import ReactorModel.Execution.Theorems.Trivial
+
+noncomputable section
+open ReactorType Classical
+
+namespace Execution.State.Over
+
+variable [Proper α] [ReactorType.Finite α]{rtr rtr₁ : α} {s : State.Over rtr}
+
+theorem exists_allowed_of_acyclic_has_unprocessed 
+    (a : Dependency.Acyclic rtr) (h₁ : i ∈ s.rtr[.rcn]) (h₂ : i ∉ s.progress) : ∃ i, s.Allows i :=
+  if h : dependencies s.rtr i \ s.progress = ∅ then
+    ⟨i, ‹_›, Set.diff_eq_empty.mp h, ‹_›⟩
+  else
+    have ⟨_, hd⟩ := Set.nonempty_iff_ne_empty.mpr h
+    have ⟨h₁, h₂⟩ := Set.mem_diff _ |>.mp hd
+    have := inferInstanceAs $ ReactorType.Finite α
+    exists_allowed_of_acyclic_has_unprocessed a h₁.mem₁ h₂
+termination_by exists_allowed_of_acyclic_has_unprocessed s i _ _ _ => 
+  have fin := Set.Finite.diff (Finite.fin s.rtr .rcn |>.subset $ dependencies_subset _ i) s.progress
+  fin.toFinset.card
+decreasing_by
+  simp_wf
+  refine Finset.card_lt_card $ Set.Finite.toFinset_strictMono ?_
+  have h := mem_dependencies_ssubset a $ s.rtr_eq ▸ h₁
+  simp [ssubset_iff_subset_ne, s.rtr_eq] at h ⊢ 
+  refine ⟨?subset, ?ne⟩
+  case subset =>
+    intro x hx
+    simp [Set.mem_diff] at hx ⊢ 
+    exact ⟨h.left hx.left, hx.right⟩
+  case ne =>
+    simp [Set.ext_iff]
+    refine ⟨_, h₂, ?_⟩
+    rw [iff_true_right $ s.rtr_eq ▸ h₁]
+    exact a _
+
+theorem progress_ssubset_of_not_closed (hc : ¬s.Closed) : s.progress ⊂ s.rtr[.rcn].ids :=
+  Set.ssubset_iff_subset_ne.mpr ⟨s.progress_sub, hc⟩
+
+theorem exists_unprocessed_of_not_closed (hc : ¬s.Closed) : ∃ i ∈ s.rtr[.rcn], i ∉ s.progress := by
+  have ⟨i, _, _⟩ := Set.exists_of_ssubset $ s.progress_ssubset_of_not_closed hc
+  exists i 
+
+-- TODO: separate proof and definitions here
+def allowed (a : Dependency.Acyclic rtr) (hc : ¬s.Closed) : { i : ID // s.Allows i } :=
+  -- have ⟨_, hi₁, hi₂⟩ := s.exists_unprocessed_of_not_closed hc
+  sorry -- exists_allowed_of_acyclic_has_unprocessed a hi₁ hi₂
+
+def ofStep {s₁ : State.Over rtr₁} {s₂ : State α} (e : s₁ ↓ s₂) : State.Over s₂.rtr := 
+  { s₂ with 
+    progress_sub := by 
+      sorry
+      -- simp [e.progress_eq, ←Equivalent.obj?_rcn_eq e.equiv]
+      -- exact Set.insert_subset.mpr ⟨e.allows_rcn.mem, s₁.progress_sub⟩ 
+    events_sub := by
+      sorry
+  }
+
+end Execution.State.Over
